$$
\begin{array}{rl}
(1)  & \displaystyle \int a^x \, dx = \frac{a^x}{\ln a} + C \\
(2)  & \displaystyle \int \sec^2 x \, dx = \tan x + C \\
(3)  & \displaystyle \int -\csc^2 x \, dx = \cot x + C \\
(4)  & \displaystyle \int \sec x \cdot \cot x \, dx = -\csc x + C \\
(5)  & \displaystyle \int \frac{1}{1 + x^2} \, dx = \arctan x + C \\
(6)  & \displaystyle \int \frac{dx}{a^2 + x^2} = \frac{1}{a} \arctan \frac{x}{a} + C \\
(7)  & \displaystyle \int \sec^2 x \, dx = \tan x + C \\
(8)  & \displaystyle \int \sec x \tan x \, dx = \sec x + C \\
(9)  & \displaystyle \int \frac{1}{\sqrt{1 - x^2}} \, dx = \arcsin x + C \\
(10) & \displaystyle \int \frac{dx}{\sqrt{a^2 - x^2}} = \arcsin \frac{x}{a} + C \\
(11) & \displaystyle \int \frac{dx}{x^2 - a^2} = \frac{1}{2a} \ln \left| \frac{x - a}{x + a} \right| + C \\
(12) & \displaystyle \int \frac{dx}{\sqrt{x^2 - a^2}} = \ln \left| x + \sqrt{x^2 - a^2} \right| + C \\
(13) & \displaystyle \int \csc x \, dx = -\ln \left| \csc x + \cot x \right| + C
\end{array}
$$

$e^x的展开式$$$e^x = \sum_{n=0}^{\infty} \frac{x^n}{n!} = 1 + x + \frac{x^2}{2!} + \frac{x^3}{3!} + \cdots + \frac{x^n}{n!} + o(x^n)$$
$$\sin(x) = \sum_{n=0}^{\infty} (-1)^n \frac{x^{2n+1}}{(2n+1)!} = x - \frac{x^3}{3!} + \frac{x^5}{5!} - \frac{x^7}{7!} + \cdots + (-1)^n \frac{x^{2n+1}}{(2n+1)!} + o(x^{2n+1})
$$